Final version

del_first_line.py
@@ -1,0 +1,6 @@
+#!/usr/bin/python
+
+import sys
+
+file_name = str(sys.argv[1])
+
